
\section*{Aufgabe 2}

\subsection*{Formel in CNF umwandeln)}

$\varphi = ( \neg X_0 \vee X_4 ) \wedge (\neg X_1 \vee (\neg X_3 \wedge X_2))$ Ist in NNF.\\

BaseStep:\\

$ \bigwedge ( \bigvee ( \neg X_0 ) ) , \bigwedge ( \bigvee (\neg X_1 ) ) , \bigwedge ( \bigvee (X_2 ) ) , \bigwedge ( \bigvee (\neg X_3 ) ) , \bigwedge ( \bigvee (X_4 ) )  $\\

Inductive step 1 $X_0 \vee X_4$:\\

$  \bigwedge ( \bigvee ( \neg X_0 , X_4 ) )  , \bigwedge ( \bigvee (\neg X_1 ) ) , \bigwedge ( \bigvee (X_2 ) ) , \bigwedge ( \bigvee (\neg X_3 ) )  $\\

Inductive step 2 $\neg X_3 \wedge X_2$:\\

$ \bigwedge ( \bigvee ( \neg X_0 , X_4 ) ) 
, \bigwedge ( \bigvee (\neg X_1 ) ) ,
 \bigwedge ( \bigvee (X_2 ),  \bigvee ( \neg X_3 )) ) ,
 $

Inductive step 3 $neg X_1 \vee ( \neg X_3 \wedge X_2 )$:\\

$ \bigwedge ( \bigvee ( \neg X_0 , X_4 ) ) 
, \bigwedge ( \bigvee (\neg X_1, X_2  ) , \bigvee (\neg X_1, \neg X_3  ) ) 
 $

Inductive step 4 $ ( \neg X_0 \vee X_4 ) \wedge (\neg X_1 \vee (\neg X_3 \wedge X_2))$:\\

$ \bigwedge ( \bigvee ( \neg X_0 , X_4 ) , \bigvee (\neg X_1, X_2  ) , \bigvee (\neg X_1, \neg X_3  ) ) 
 $

